

# 1 Tutorial Week 9-10: Ito formula and Black-Scholes Formula

1. Let  $W_t$  denote a Brownian motion. Use Ito's formula to compute the differentials of the following stochastic processes:

- a)  $X_t = e^{\frac{1}{2}t} \cos(W_t)$
- b)  $X_t = e^{\frac{1}{2}t} \sin(W_t)$
- c)  $X_t = (W_t + t) e^{-W_t - \frac{1}{2}t}$

2. a) Show that the price of the option with payoff

$$h(S_T) = S_T \log\left(\frac{S_T}{K}\right)$$

with  $K > 0$  at time  $t$  given  $S_t = x$  is given by

$$V(t, x) = x \left( \log\left(\frac{x}{K}\right) + \left(r + \frac{1}{2}\sigma^2\right)(T - t) \right)$$

where  $r$  is the interest rate and  $\sigma$  the volatility.

b) Compute Greeks of this option, i.e. compute the derivatives  $\frac{\partial}{\partial x} V(t, x)$ ,  $\frac{\partial^2}{\partial x^2} V(t, x)$  and  $\frac{\partial}{\partial \sigma} V(t, x)$

3. Consider the stock price process  $S_t$  under the Black and Scholes assumption, that is,  $S_t = S_0 \exp\left((r - \frac{1}{2}\sigma^2)t + \sigma W_t\right)$ , where  $W_t$  is the Wiener process under the martingale measure  $\tilde{\mathbb{P}}$ . Compute the expectation of the Asian underlying, i.e.

$$\mathbb{E}_{\tilde{\mathbb{P}}} \left( \frac{1}{T} \int_0^T S_t dt \right).$$

Hint: Use that the expectation operator  $\mathbb{E}$  and the integral  $\int_0^T$  can be interchanged.

# 2 Solution to Tutorial Week 9-10

1.

a) Recall formulation of Ito formula from lectures:

For the process

$$dx(t) = \phi(t, x(t)) dt + \sigma(t, x(t)) dW(t)$$

take a composite function

$$g(t) = G(t, x(t))$$

then its process is

$$\begin{aligned} dg(t) = & \left( G_t(t, x(t)) + G_x(t, x(t)) \phi(t, x(t)) + \frac{1}{2} G_{xx}(t, x(t)) \sigma^2(t, x(t)) \right) dt \\ & + G_x(t, x(t)) \sigma(t, x(t)) dW(t) \end{aligned}$$

so it is a general formula how to differentiate composite functions.

Now, we need to understand "what is what" in  $X_t = \exp\left(\frac{1}{2}t\right) \cos(W_t)$

An obvious way:

$$\begin{aligned} x(t) &= W(t) \\ \sigma(t, x(t)) &= 1 \\ \phi(t, x(t)) &= 0 \\ g(t) &= G(t, x(t)) = \exp\left(\frac{1}{2}t\right) \cos(x(t)) \end{aligned}$$

Then only three terms remain in Ito formula once we substitute  $\sigma = 1$  and  $\phi = 0$  :

$$dg(t) = \left( G_t(t, x(t)) + \frac{1}{2} G_{xx}(t, x(t)) \right) dt + G_x(t, x(t)) dW(t)$$

And we need to find these partial derivatives. The approach is the same for all three cases.

a)  $X_t = e^{\frac{1}{2}t} \cos(W_t)$

$$X_t = G(t, W_t) = e^{\frac{1}{2}t} \cos(W_t)$$

$$\begin{aligned} \frac{\partial G(t, W_t)}{\partial t} &= \frac{1}{2} e^{\frac{1}{2}t} \cos(W_t) \\ \frac{\partial G(t, W_t)}{\partial W} &= -e^{\frac{1}{2}t} \sin(W_t) \\ \frac{\partial^2 G(t, W_t)}{\partial W^2} &= -e^{\frac{1}{2}t} \cos(W_t) \end{aligned}$$

$$\begin{aligned} dX_t &= \frac{1}{2} e^{\frac{1}{2}t} \cos(W_t) dt - e^{\frac{1}{2}t} \sin(W_t) dW_t - \frac{1}{2} e^{\frac{1}{2}t} \cos(W_t) dt \\ &= -e^{\frac{1}{2}t} \sin(W_t) dW_t \end{aligned}$$

b)  $X_t = e^{\frac{1}{2}t} \sin(W_t)$

$$G(t, W_t) = e^{\frac{1}{2}t} \sin(W_t)$$

$$\begin{aligned} \frac{\partial G(t, W_t)}{\partial t} &= \frac{1}{2} e^{\frac{1}{2}t} \sin(W_t) \\ \frac{\partial G(t, W_t)}{\partial W} &= e^{\frac{1}{2}t} \cos(W_t) \\ \frac{\partial^2 G(t, W_t)}{\partial W^2} &= -e^{\frac{1}{2}t} \sin(W_t) \end{aligned}$$

$$\begin{aligned} dX_t &= \frac{1}{2} e^{\frac{1}{2}t} \sin(W_t) dt + e^{\frac{1}{2}t} \cos(W_t) dW_t - \frac{1}{2} e^{\frac{1}{2}t} \sin(W_t) dt \\ &= e^{\frac{1}{2}t} \cos(W_t) dW_t \end{aligned}$$

c)  $X_t = (W_t + t) e^{-W_t - \frac{1}{2}t}$

$$G(t, W_t) = (W_t + t) e^{-W_t - \frac{1}{2}t}$$

$$\begin{aligned}\frac{\partial G(t, W_t)}{\partial t} &= e^{-W_t - \frac{1}{2}t} - \frac{1}{2} (W_t + t) e^{-W_t - \frac{1}{2}t} \\ \frac{\partial G(t, W_t)}{\partial W} &= e^{-W_t - \frac{1}{2}t} - (W_t + t) e^{-W_t - \frac{1}{2}t} \\ \frac{\partial^2 G(t, W_t)}{\partial W^2} &= -e^{-W_t - \frac{1}{2}t} - e^{-W_t - \frac{1}{2}t} + (W_t + t) e^{-W_t - \frac{1}{2}t}\end{aligned}$$

$$\begin{aligned}dX_t &= \left( e^{-W_t - \frac{1}{2}t} - \frac{1}{2} (W_t + t) e^{-W_t - \frac{1}{2}t} \right) dt + \left( e^{-W_t - \frac{1}{2}t} - (W_t + t) e^{-W_t - \frac{1}{2}t} \right) dW_t \\ &\quad + \frac{1}{2} \left( -e^{-W_t - \frac{1}{2}t} - e^{-W_t - \frac{1}{2}t} + (W_t + t) e^{-W_t - \frac{1}{2}t} \right) dt \\ &= (1 - W_t - t) e^{-W_t - \frac{1}{2}t} dW_t\end{aligned}$$

2. a) First, check that

$$V(T, S_T) = S_T \left( \log \left( \frac{S_T}{K} \right) + \left( r + \frac{1}{2} \sigma^2 \right) (T - T) \right) = S_T \log \left( \frac{S_T}{K} \right) = h(S_T)$$

so the terminal condition is verified

Second, check that

$$V(t, x) = x \left( \log \left( \frac{x}{K} \right) + \left( r + \frac{1}{2} \sigma^2 \right) (T - t) \right)$$

satisfies Black-Scholes equation

$$rV(t, x) - \frac{\partial}{\partial t} V(t, x) = \frac{\sigma^2 x^2}{2} \frac{\partial^2}{\partial x^2} V(t, x) + rx \frac{\partial}{\partial x} V(t, x),$$

$$\begin{aligned}\frac{\partial V(t, x)}{\partial t} &= -x \left( r + \frac{1}{2} \sigma^2 \right) \\ \frac{\partial V(t, x)}{\partial x} &= \left( \log \left( \frac{x}{K} \right) + \left( r + \frac{1}{2} \sigma^2 \right) (T - t) \right) + x \frac{1}{x} = \log \left( \frac{x}{K} \right) + \left( r + \frac{1}{2} \sigma^2 \right) (T - t) + 1 \\ \frac{\partial^2 V(t, x)}{\partial x^2} &= \frac{1}{x}\end{aligned}$$

$$\begin{aligned}rx \left( \log \left( \frac{x}{K} \right) + \left( r + \frac{1}{2} \sigma^2 \right) (T - t) \right) + x \left( r + \frac{1}{2} \sigma^2 \right) &= \frac{\sigma^2 x^2}{2} \frac{1}{x} + rx \left( \log \left( \frac{x}{K} \right) + \left( r + \frac{1}{2} \sigma^2 \right) (T - t) + 1 \right) \\ rx \log \left( \frac{x}{K} \right) + rx \left( r + \frac{1}{2} \sigma^2 \right) (T - t) + x \left( r + \frac{1}{2} \sigma^2 \right) &= \frac{\sigma^2}{2} x + rx \log \left( \frac{x}{K} \right) + rx \left( r + \frac{1}{2} \sigma^2 \right) (T - t) + rx\end{aligned}$$

which is easily verified.

b) Compute Greeks of this option

$$\begin{aligned}
\Delta &= \frac{\partial V(t, x)}{\partial x} = \log\left(\frac{x}{K}\right) + \left(r + \frac{1}{2}\sigma^2\right)(T - t) + 1 \\
\Theta &= \frac{\partial V(t, x)}{\partial t} = -x \left(r + \frac{1}{2}\sigma^2\right) \\
\Gamma &= \frac{\partial^2 V(t, x)}{\partial x^2} = \frac{1}{x} \\
\rho &= \frac{\partial V(t, x)}{\partial r} = x(T - t) \\
vega &= \frac{\partial V(t, x)}{\partial \sigma} = x\sigma(T - t)
\end{aligned}$$

3.

$$\begin{aligned}
\mathbb{E}_{\tilde{\mathbb{P}}}\left(\frac{1}{T} \int_0^T S_t dt\right) &= \mathbb{E}_{\tilde{\mathbb{P}}}\left(\frac{1}{T} \int_0^T S_0 \exp\left(\left(r - \frac{1}{2}\sigma^2\right)t + \sigma W_t\right) dt\right) \\
&= \frac{S_0}{T} \int_0^T \mathbb{E}_{\tilde{\mathbb{P}}}\left(e^{(r - \frac{1}{2}\sigma^2)t} e^{\sigma W_t}\right) dt \\
&= \frac{S_0}{T} \int_0^T e^{(r - \frac{1}{2}\sigma^2)t} \mathbb{E}_{\tilde{\mathbb{P}}}\left(e^{\sigma W_t}\right) dt \\
&= \frac{S_0}{T} \int_0^T e^{(r - \frac{1}{2}\sigma^2)t} \mathbb{E}_{\tilde{\mathbb{P}}}\left(e^{\sigma(W_t - W_0)} e^{\sigma(W_0)}\right) dt
\end{aligned}$$

Now,  $W_0 = 0$  and  $(W_t - W_0) \sim N(0, \sqrt{t})$  so that

$$\mathbb{E}_{\tilde{\mathbb{P}}}\left(\frac{1}{T} \int_0^T S_t dt\right) = \frac{S_0}{T} \int_0^T e^{(r - \frac{1}{2}\sigma^2)t} \mathbb{E}_{\tilde{\mathbb{P}}}\left(e^{\sigma(W_t - W_0)}\right) dt$$

We need to compute  $\mathbb{E}_{\tilde{\mathbb{P}}}\left(e^{\sigma(W_t - W_0)}\right)$

$(W_t - W_0) \sim N(0, \sqrt{t})$ , or  $\sigma(W_t - W_0) \sim N(0, \sigma\sqrt{t})$

We have general formula for the mean of log-normal distribution

Recall that

$$\mathbb{E}_{\tilde{\mathbb{P}}}\left(e^{\mu + \sigma Z}\right) = e^{\mu + \frac{1}{2}\sigma^2}$$

where  $Z \sim N(0, 1)$

We have

$$\sigma(W_t - W_0) = 0 + \sigma\sqrt{t}Z$$

and

$$\mathbb{E}_{\tilde{\mathbb{P}}}\left(e^{\sigma\sqrt{t}Z}\right) = e^{\frac{1}{2}\sigma^2 t}$$

so that

$$\begin{aligned}\mathbb{E}_{\tilde{\mathbb{P}}}\left(\frac{1}{T}\int_0^T S_t dt\right) &= \frac{S_0}{T}\int_0^T e^{(r-\frac{1}{2}\sigma^2)t}e^{\frac{1}{2}\sigma^2 t}dt \\ &= \frac{S_0}{T}\int_0^T e^{rt}dt \\ &= \frac{S_0}{Tr}(e^{rT}-1)\end{aligned}$$